Improve SimI structure

theories/Equiv/SimI.v
@@ -25,31 +25,118 @@ Class ProofRelationI (A:Type) := {
 Definition irel := rel3 simtype (fun _ : simtype => I.state)
                        (fun (_ : simtype) (_ : I.state) => I.state).
 
-Definition simILabenv t (r:irel)
-           {A} (PR:ProofRelationI A) (AL:list A) L L' :=
-  (length AL = length L /\ sawtooth L' /\ sawtooth L) /\
-  forall f f' a Z s n Z' s' n',
-    IndexRelI AL (counted f) (counted f')
-    -> get AL (counted f) a
-    -> get L (counted f) (I.blockI Z s n)
-    -> get L' (counted f') (I.blockI Z' s' n')
-    -> (ParamRelI a Z Z')
-      /\ (forall E E' Yv Y'v Y Y',
-            ArgRelI E E' a Yv Y'v
-            -> omap (exp_eval E) Y = Some Yv
-            -> omap (exp_eval E') Y' = Some Y'v
-            -> sim'r r t (L, E, stmtApp f Y)
-                    (L', E', stmtApp f' Y')).
+Coercion labN : lab >-> nat.
 
-Lemma simILabenv_mon t (r r':irel) A (PR:ProofRelationI A) AL L L'
-  : simILabenv t r PR AL L L'
+Definition paramrel A (PR:ProofRelationI A) AL L L' :=
+  forall (f f':lab) Z s i Z' s' i' a,
+    IndexRelI AL f f'
+    -> get AL f a
+    -> get L f (I.blockI Z s i)
+    -> get L' f' (I.blockI Z' s' i')
+    -> ParamRelI a Z Z'.
+
+Definition app_r t (r:irel) A (PR:ProofRelationI A) AL (L L':I.labenv) :=
+  forall (f f':lab) a Z s i Z' s' i',
+    IndexRelI AL f f'
+    -> get AL f a
+    -> get L f (I.blockI Z s i)
+    -> get L' f' (I.blockI Z' s' i')
+    -> forall E E' Yv Y'v Y Y',
+        ArgRelI E E' a Yv Y'v
+        -> omap (exp_eval E) Y = Some Yv
+        -> omap (exp_eval E') Y' = Some Y'v
+        -> r t (L, E, stmtApp f Y)
+            (L', E', stmtApp f' Y').
+
+Lemma app_r_mon t (r r':irel) A (PR:ProofRelationI A) AL L L'
+  : app_r t r PR AL L L'
     -> (forall t x y, r t x y -> r' t x y)
-    -> simILabenv t r' PR AL L L'.
+    -> app_r t r' PR AL L L'.
 Proof.
-  intros [[? ?] SIM] LE; hnf; intros; split; eauto.
-  intros. edestruct SIM as [? SIM']; eauto.
-  split; eauto. intros.
-  eapply paco3_mon. eapply SIM; eauto. eauto.
+  intros Lr LE; hnf; intros; eauto.
+Qed.
+
+Definition labenv_sim t (r:irel)
+           {A} (PR:ProofRelationI A) (AL:list A) L L' :=
+  length AL = length L /\
+  sawtooth L' /\
+  sawtooth L /\
+  paramrel PR AL L L' /\
+  app_r t r PR AL L L'.
+
+Lemma labenv_sim_nil t r A PR
+  : @labenv_sim t r A PR nil nil nil.
+Proof.
+  repeat split; eauto using @sawtooth.
+  hnf; intros; isabsurd.
+  hnf; intros; isabsurd.
+Qed.
+
+Hint Immediate labenv_sim_nil.
+
+Lemma labenv_sim_mon t (r r':irel) A (PR:ProofRelationI A) AL L L'
+  :  labenv_sim t r PR AL L L'
+    -> (forall t x y, r t x y -> r' t x y)
+    -> labenv_sim t r' PR AL L L'.
+Proof.
+  intros [LEN [STL [STL' [PAR SIM]]]] LE; hnf; repeat split; eauto.
+  eapply app_r_mon; eauto.
+Qed.
+
+Definition bodies_r t (r:irel) A (PR:ProofRelationI A) AL (L1 L2 L L':I.labenv) :=
+  forall f f' Z s i Z' s' i' a,
+    IndexRelI AL f f'
+    -> get L f (I.blockI Z s i)
+    -> get L' f' (I.blockI Z' s' i')
+    -> get AL f a
+    -> forall E E' VL VL',
+        ArgRelI E E' a VL VL'
+        -> r t (drop (f - i) L1, E[Z <-- List.map Some VL], s)
+            (drop (f' - i') L2, E'[Z' <-- List.map Some VL'], s').
+
+Lemma bodies_r_mon t (r r':irel) A (PR:ProofRelationI A) AL L1 L2 L L'
+  : bodies_r t r PR AL L1 L2 L L'
+    -> (forall t x y, r t x y -> r' t x y)
+    -> bodies_r t r' PR AL L1 L2 L L'.
+Proof.
+  intros Idx LE; hnf; intros; eauto.
+Qed.
+
+Lemma fix_compatible_bodies t A (PR:ProofRelationI A) AL L L'
+  : (forall r L1 L2, app_r t (sim'r r) PR AL L1 L2
+          -> bodies_r t (sim'r r) PR AL L1 L2 L L')
+    -> paramrel PR AL L L'
+    -> forall r, bodies_r t (sim'r r) PR AL L L' L L'.
+Proof.
+  intros ISIM LP r. pcofix CIH.
+  eapply ISIM.
+  hnf; intros.
+  exploit LP; eauto.
+  exploit ArgLengthMatchI; eauto; dcr.
+  pone_step; simpl; eauto with len.
+Qed.
+
+Lemma stepGoto_mapi L blk Y E vl f F k
+      (Ldef:get L (counted f - ❬F❭) blk)
+      (len:length (I.block_Z blk) = length Y)
+      (def:omap (exp_eval E) Y = Some vl) E'
+      (updOk:E [I.block_Z blk <-- List.map Some vl] = E')
+      (ST:smaller L) (GE: counted f >= ❬F❭) (EQ:k = counted f - ❬F❭ - block_n blk)
+  : I.step (mapi I.mkBlock F ++ L, E, stmtApp f Y) EvtTau
+           (drop k L,
+            E', I.block_s blk).
+Proof.
+  subst.
+  rewrite <- (mapi_length I.mkBlock).
+  assert (counted f - block_n blk >= ❬mapi I.mkBlock F❭). {
+    exploit (ST _ _ Ldef).
+    rewrite mapi_length. simpl in *. omega.
+  }
+  orewrite (counted f - ❬mapi I.mkBlock F❭ - block_n blk
+            =  (counted f - block_n blk) - ❬mapi I.mkBlock F❭).
+  rewrite <- (drop_app_gen _ (mapi I.mkBlock F)); eauto.
+  eapply I.stepGoto; eauto.
+  rewrite get_app_ge. rewrite mapi_length. eauto. omega.
 Qed.
 
 Definition indexwise_r t (r:irel) A (PR:ProofRelationI A) AL' F F' AL L L' :=
@@ -60,8 +147,8 @@ Definition indexwise_r t (r:irel) A (PR:ProofRelationI A) AL' F F' AL L L' :=
     -> get AL' n a
     -> forall E E' VL VL',
         ArgRelI E E' a VL VL'
-        -> r t (mapi I.mkBlock F ++ L, E[Z <-- List.map Some VL], s)
-            (mapi I.mkBlock F' ++ L', E'[Z' <-- List.map Some VL'], s').
+        -> r t (L, E[Z <-- List.map Some VL], s)
+            (L', E'[Z' <-- List.map Some VL'], s').
 
 Lemma indexwise_r_mon t (r r':irel) A (PR:ProofRelationI A) AL' F F' AL L L'
   : indexwise_r t r PR AL' F F' AL L L'
@@ -71,7 +158,7 @@ Proof.
   intros Idx LE; hnf; intros; eauto.
 Qed.
 
-Definition indexwise_proofrel A (PR:ProofRelationI A) (F F':〔params * stmt〕) AL' AL :=
+Definition indexwise_paramrel A (PR:ProofRelationI A) (F F':〔params * stmt〕) AL' AL :=
   forall n n' Z s Z' s' a,
     IndexRelI (AL' ++ AL) n n'
     -> get F n (Z,s)
@@ -79,133 +166,215 @@ Definition indexwise_proofrel A (PR:ProofRelationI A) (F F':〔params * stmt〕)
     -> get AL' n a
     -> ParamRelI a Z Z'.
 
-Lemma stepGoto_mapi L blk Y E vl f F
-      (Ldef:get L (counted f - ❬F❭) blk)
-      (len:length (I.block_Z blk) = length Y)
-      (def:omap (exp_eval E) Y = Some vl) E'
-      (updOk:E [I.block_Z blk <-- List.map Some vl] = E')
-      (ST:sawtooth L) (GE: counted f >= ❬F❭)
-  : I.step (mapi I.mkBlock F ++ L, E, stmtApp f Y) EvtTau
-           (drop (counted f - ❬F❭ - block_n blk) L,
-            E', I.block_s blk).
+Definition separates A (PR:ProofRelationI A) AL' AL (F F':〔params * stmt〕) :=
+  length AL' = length F
+  /\ Image AL' = length F'
+  /\ (forall n n', IndexRelI (AL' ++ AL) n n' -> n < length F -> n' < length F')
+  /\  (forall n n', IndexRelI (AL' ++ AL) n n' -> n >= length F -> n' >= length F').
+
+Lemma complete_paramrel A (PR:ProofRelationI A) F F' AL' AL L L'
+  : indexwise_paramrel PR F F' AL' AL
+    -> paramrel PR AL L L'
+    -> separates PR AL' AL F F'
+    -> paramrel PR (AL' ++ AL) (mapi I.mkBlock F ++ L) (mapi I.mkBlock F' ++ L').
 Proof.
-  rewrite <- (mapi_length I.mkBlock).
-  assert (counted f - block_n blk >= ❬mapi I.mkBlock F❭). {
-    exploit (sawtooth_smaller ST Ldef).
-    rewrite mapi_length. simpl in *. omega.
-  }
-  orewrite (counted f - ❬mapi I.mkBlock F❭ - block_n blk
-            =  (counted f - block_n blk) - ❬mapi I.mkBlock F❭).
-  rewrite <- (drop_app_gen _ (mapi I.mkBlock F)); eauto.
-  eapply I.stepGoto; eauto.
-  rewrite get_app_ge. rewrite mapi_length. eauto. omega.
+  intros IPR PAR [Len1 [Img [Ilt Ige]]].
+  hnf; intros ? ? ? ? ? ? ? ? ? RN GetAL GetFL GetL'.
+  eapply get_app_cases in GetFL; destruct GetFL as [GetFL'| [GetFL GE]].
+  - exploit Ilt; eauto. eapply get_range in GetFL'.
+    rewrite mapi_length in GetFL'; eauto.
+    eapply get_app_lt_1 in GetL'; [| rewrite mapi_length; eauto ].
+    inv_get. destruct x0 as [Z s], x as [Z' s']. simpl in *. clear EQ0 EQ.
+    eauto.
+  - rewrite mapi_length in *; eauto.
+    exploit Ige; eauto.
+    eapply get_app_right_ge in GetAL; [ | rewrite Len1; eauto ].
+    eapply get_app_right_ge in GetL'; [ | rewrite mapi_length; eauto ].
+    eapply IndexRelDrop in RN; [| rewrite Len1; rewrite mapi_length in *; eauto].
+    exploit (PAR (LabI  (f - ❬AL'❭)) (LabI (f' - Image AL'))); eauto.
+    rewrite Len1; eauto. rewrite Img; rewrite mapi_length in *; eauto.
 Qed.
 
-Lemma simILabenv_extension' t (r:irel) A (PR:ProofRelationI A) (AL AL':list A) F F' L L'
-      (LEN1:length AL' = length F)
-  : indexwise_r t (sim'r r \3/ r) PR AL' F F' AL L L'
-    -> indexwise_proofrel PR F F' AL' AL
-    -> (forall n n', IndexRelI (AL' ++ AL) n n' -> n < length AL' -> n' < Image AL')
-    -> (forall n n', IndexRelI (AL' ++ AL) n n' -> n >= length AL' -> n' >= Image AL')
-    -> Image AL' = length F'
-    -> simILabenv t r PR AL L L'
-    -> simILabenv t r PR (AL' ++ AL) (mapi I.mkBlock F ++ L) (mapi I.mkBlock F' ++ L').
+Hint Unfold separates.
+
+Lemma labenv_sim_extension' t r A (PR:ProofRelationI A) (AL AL':list A) F F' L L'
+  : indexwise_r t (sim'r r \3/ r) PR AL' F F' AL (mapi I.mkBlock F ++ L) (mapi I.mkBlock F' ++ L')
+    -> indexwise_paramrel PR F F' AL' AL
+    -> separates PR AL' AL F F'
+    -> labenv_sim t (sim'r r) PR AL L L'
+    -> labenv_sim t (sim'r r) PR (AL' ++ AL) (mapi I.mkBlock F ++ L) (mapi I.mkBlock F' ++ L').
 Proof.
-  intros ISIM IP Ilt Ige Img SIML.
-  hnf. split.
-  destruct SIML; dcr; split; eauto with len. split; eauto.
-  econstructor; eauto. eapply tooth_I_mkBlocks.
-  econstructor; eauto. eapply tooth_I_mkBlocks.
+  intros SIM IPR [Len2 [Img [Ilt Ige]]] [Len1 [STL [STL' [PAR LSIM]]]].
+  hnf; repeat split; eauto 20 using sawtooth_I_mkBlocks, complete_paramrel with len.
   intros f f' ? ? ? ? ? ? ? RN GetAL GetFL GetL'.
-  assert (❬AL'❭ = ❬mapi I.mkBlock F❭) by eauto with len.
-  eapply get_app_cases in GetAL. destruct GetAL as [GetAL'|GetAL].
-  - eapply get_app_lt_1 in GetFL; [| rewrite <- H; eauto using get_range].
-    inv_get. destruct x as [Z s]. simpl in *. clear EQ.
-    exploit Ilt; eauto using get_range. rewrite Img in H0.
-    eapply get_app_lt_1 in GetL'; [| rewrite mapi_length; eauto with len ].
-    inv_get. destruct x as [Z' s']; simpl in *; clear EQ.
-    split; eauto.
-    intros.
+  assert (Len3:❬AL'❭ = ❬mapi I.mkBlock F❭) by eauto with len.
+  eapply get_app_cases in GetFL. destruct GetFL as [GetFL'| [GetFL GE]].
+  - exploit Ilt; eauto. eapply get_range in GetFL'.
+    rewrite mapi_length in GetFL'; eauto.
+    eapply get_app_lt_1 in GetL'; [| rewrite mapi_length; eauto ].
+    inv_get. destruct x0 as [Z s], x as [Z' s']. simpl in *. clear EQ0 EQ.
+    exploit IPR; eauto.
     exploit (ArgLengthMatchI); eauto; dcr.
-    pone_step; eauto using get_app, get_mapi; eauto; simpl; eauto with len.
-    orewrite (labN f - labN f = 0); simpl.
-    orewrite (labN f' - labN f' = 0); simpl.
-    eapply ISIM; eauto.
-  - destruct SIML; dcr.
-    eapply get_app_right_ge in GetFL; [ | rewrite <- H; eauto].
-    exploit Ige; eauto; try congruence.
-    eapply get_app_right_ge in GetL'; [ | eauto with len; rewrite mapi_length; eauto].
+    pone_step; simpl; eauto using get_app, get_mapi; simpl; eauto with len.
+    orewrite (f-f=0). orewrite (f'-f'=0). simpl.
+    exploit SIM; eauto.
+  - exploit Ige; eauto. rewrite mapi_length in GE; eauto.
+    eapply get_app_right_ge in GetAL; [ | rewrite Len3; eauto ].
+    eapply get_app_right_ge in GetL'; [ | rewrite mapi_length; eauto ].
     rewrite mapi_length in *.
-    eapply IndexRelDrop in RN; eauto.
-    edestruct (H1 (LabI (counted f - ❬AL'❭)) (LabI (counted f' - Image AL')))
-      as [? SIM]; simpl; eauto.
-    rewrite H; eauto. rewrite Img; eauto.
-    split; eauto.
-    intros.
+    eapply IndexRelDrop in RN; eauto; [| rewrite Len3; eauto].
+    exploit (LSIM (LabI  (f - ❬AL'❭)) (LabI (f' - Image AL'))) as SIMR; eauto.
+    rewrite Len3; eauto. rewrite Img; eauto.
+    exploit (PAR (LabI  (f - ❬AL'❭)) (LabI (f' - Image AL'))); eauto.
+    rewrite Len3; eauto. rewrite Img; eauto.
     exploit (ArgLengthMatchI); eauto; dcr.
     eapply (@sim_Y_left I.state _ I.state _).
     eapply (@sim_Y_right I.state _ I.state _).
-    rewrite Img in SIM. rewrite H in SIM.
-    eapply SIM; eauto.
+    rewrite Img in SIMR. rewrite Len3 in SIMR.
+    eapply paco3_mon; [| eauto].
+    eapply SIMR; eauto.
     econstructor; simpl; eauto with len. simpl. eauto with len.
-    Focus 2.
+    eapply stepGoto_mapi; simpl in *; eauto using @sawtooth_smaller with len.
     econstructor; simpl; eauto. simpl. eauto with len.
-    simpl.
-    eapply (stepGoto_mapi _ _ _ _ GetL'); simpl; eauto with len. rewrite
-    eapply (stepGoto_mapi _ _ _ _ GetFL); simpl; eauto with len.
-    simpl in *; omega.
+    eapply stepGoto_mapi; simpl in *; eauto using @sawtooth_smaller with len.
 Qed.
 
-Lemma fix_compatible_I t A (PR:ProofRelationI A) AL F F' L L' AL'
-(LEN2:length AL' = length F)
-  : (forall r, simILabenv t r PR (AL' ++ AL) (mapi I.mkBlock F ++ L)
-                     (mapi I.mkBlock F' ++ L')
-            -> indexwise_r t (sim'r r) PR AL' F F' AL L L')
+(*
+Lemma labenv_sim_extension' t A (PR:ProofRelationI A) (AL AL':list A) F F' L L'
+  : (forall r L1 L2, labenv_sim t (sim'r r) PR (AL' ++ AL) L1 L2
+                -> indexwise_r t (sim'r r) PR AL' F F' AL L1 L2)
     -> indexwise_proofrel PR F F' AL' AL
-    -> (forall n n', IndexRelI (AL' ++ AL) n n' -> n < length AL' -> n' < Image AL')
-    -> (forall n n', IndexRelI (AL' ++ AL) n n' -> n >= length AL' -> n' >= Image AL')
-    -> Image AL' = length F'
-    -> forall r, simILabenv t r PR AL L L'
-           -> indexwise_r t (sim'r r) PR AL' F F' AL L L'.
+    -> separates PR AL' AL F F'
+    -> paramrel PR AL L L'
+    -> sawtooth L
+    -> sawtooth L'
+    -> forall r, labenv_sim t (sim'r r) PR AL L L'
+        -> app_r t (sim'r r) PR (AL' ++ AL) (mapi I.mkBlock F ++ L) (mapi I.mkBlock F' ++ L').
 Proof.
-  intros ISIM IP Ilt Ige Img r SIML; pcofix CIH.
+  intros SIM IPR [Len2 [Img [Ilt Ige]]] PAR STL STL' r LSIM. pcofix CIH.
+  intros f f' ? ? ? ? ? ? ? RN GetAL GetFL GetL'.
+  assert (Len1:❬AL'❭ = ❬mapi I.mkBlock F❭) by eauto with len.
+  eapply get_app_cases in GetFL. destruct GetFL as [GetFL'| [GetFL GE]].
+  - exploit Ilt; eauto. eapply get_range in GetFL'.
+    rewrite mapi_length in GetFL'; eauto.
+    eapply get_app_lt_1 in GetL'; [| rewrite mapi_length; eauto ].
+    inv_get. destruct x0 as [Z s], x as [Z' s']. simpl in *. clear EQ0 EQ.
+    exploit IPR; eauto.
+    exploit (ArgLengthMatchI); eauto; dcr.
+    exploit SIM.
+    repeat split; [ | | | | eapply app_r_mon; eauto];
+      eauto using sawtooth_I_mkBlocks, indexwise_paramrel with len.
+    hnf in LSIM; dcr; eauto with len.
+    exploit H1; eauto.
+    pone_step; simpl; eauto using get_app, get_mapi; simpl; eauto with len.
+    left.
+    orewrite (f-f=0). orewrite (f'-f'=0). simpl.
+    exploit H0; eauto.
+  - exploit Ige; eauto. rewrite mapi_length in GE; eauto.
+    eapply get_app_right_ge in GetAL; [ | rewrite Len1; eauto ].
+    eapply get_app_right_ge in GetL'; [ | rewrite mapi_length; eauto ].
+    rewrite mapi_length in *.
+    eapply IndexRelDrop in RN; eauto; [| rewrite Len1; eauto].
+    destruct LSIM as [Len3 [STLx [STL'x [PARx LSIM]]]].
+    exploit (LSIM (LabI  (f - ❬AL'❭)) (LabI (f' - Image AL'))) as SIMR; eauto.
+    rewrite Len1; eauto. rewrite Img; eauto.
+    exploit (PAR (LabI  (f - ❬AL'❭)) (LabI (f' - Image AL'))); eauto.
+    rewrite Len1; eauto. rewrite Img; eauto.
+    exploit (ArgLengthMatchI); eauto; dcr.
+    eapply (@sim_Y_left I.state _ I.state _).
+    eapply (@sim_Y_right I.state _ I.state _).
+    rewrite Img in SIMR. rewrite Len1 in SIMR.
+    eapply paco3_mon; [| eauto].
+    eapply SIMR; eauto.
+    econstructor; simpl; eauto with len. simpl. eauto with len.
+    eapply stepGoto_mapi; simpl in *; eauto using @sawtooth_smaller with len.
+    econstructor; simpl; eauto. simpl. eauto with len.
+    eapply stepGoto_mapi; simpl in *; eauto using @sawtooth_smaller with len.
+Qed.
+ *)
+
+
+Lemma fix_compatible_separate t A (PR:ProofRelationI A) AL' AL F F' L L'
+  : (forall r,
+        labenv_sim t (sim'r r) PR (AL' ++ AL) (mapi I.mkBlock F ++ L) (mapi I.mkBlock F' ++ L')
+        -> indexwise_r t (sim'r r) PR AL' F F' AL (mapi I.mkBlock F ++ L) (mapi I.mkBlock F' ++ L'))
+    -> indexwise_paramrel PR F F' AL' AL
+    -> separates PR AL' AL F F'
+    -> forall r, labenv_sim t (sim'r r) PR AL L L'
+           -> indexwise_r t (sim'r r) PR AL' F F' AL (mapi I.mkBlock F ++ L) (mapi I.mkBlock F' ++ L').
+Proof.
+  intros ISIM LP SEP r SIML. pcofix CIH.
   eapply ISIM.
-  eapply simILabenv_extension'; eauto using simILabenv_mon, indexwise_r_mon.
+  eapply labenv_sim_extension'; eauto.
+  eauto using indexwise_r_mon; eauto.
+  eapply labenv_sim_mon; eauto.
+  intros. eapply paco3_mon; eauto.
 Qed.
 
-Lemma simILabenv_extension t A (PR:ProofRelationI A) (AL AL':list A) F F' L L'
-      (LEN1:length AL' = length F)
-  : (forall r, simILabenv t r PR (AL' ++ AL) (mapi I.mkBlock F ++ L)
-                     (mapi I.mkBlock F' ++ L')
-          -> indexwise_r t (sim'r r) PR AL' F F' AL L L')
-    -> indexwise_proofrel PR F F' AL' AL
-    -> (forall n n', IndexRelI (AL' ++ AL) n n' -> n < length F -> n' < length F')
-    -> (forall n n', IndexRelI (AL' ++ AL) n n' -> n >= length F -> n' >= length F')
-    -> Image AL' = length F'
-    -> forall r, simILabenv t r PR AL L L'
-           -> simILabenv t r PR (AL' ++ AL) (mapi I.mkBlock F ++ L) (mapi I.mkBlock F' ++ L').
+
+Lemma labenv_sim_extension t A (PR:ProofRelationI A) (AL AL':list A) F F' L L'
+  : (forall r,
+        labenv_sim t (sim'r r) PR (AL' ++ AL) (mapi I.mkBlock F ++ L) (mapi I.mkBlock F' ++ L')
+        -> indexwise_r t (sim'r r) PR AL' F F' AL (mapi I.mkBlock F ++ L) (mapi I.mkBlock F' ++ L'))
+    -> indexwise_paramrel PR F F' AL' AL
+    -> separates PR AL' AL F F'
+    -> forall r, labenv_sim t (sim'r r) PR AL L L'
+        -> labenv_sim t (sim'r r) PR (AL' ++ AL) (mapi I.mkBlock F ++ L) (mapi I.mkBlock F' ++ L').
 Proof.
-  intros. eapply simILabenv_extension'; eauto.
+  intros ISIM IP SEP r SIML.
+  eapply labenv_sim_extension'; eauto.
   eapply indexwise_r_mon.
-  eapply fix_compatible_I; eauto. eauto.
+  eapply fix_compatible_separate; eauto. eauto.
 Qed.
 
-Lemma simILabenv_extension_len t A (PR:ProofRelationI A) (AL AL':list A) F F' L L'
-      (LEN1:length AL' = length F) (LEN2:length F = length F')
-      (IDX:forall AL n n', IndexRelI AL n n' = (n = n'))
-  : (forall r, simILabenv t r PR (AL' ++ AL) (mapi I.mkBlock F ++ L)
-                     (mapi I.mkBlock F' ++ L')
-          -> indexwise_r t (sim'r r) PR AL' F F' AL L L')
-    -> indexwise_proofrel PR F F' AL' AL
-    -> Image AL' = length F'
-    -> forall r, simILabenv t r PR AL L L'
-           -> simILabenv t r PR (AL' ++ AL) (mapi I.mkBlock F ++ L) (mapi I.mkBlock F' ++ L').
+
+(* A proof relation is parameterized by analysis information A *)
+Class PointwiseProofRelationI (A:Type) := {
+    (* Relates parameter lists according to analysis information *)
+    ParamRelIP : A -> list var -> list var -> Prop;
+    (* Relates argument lists according to analysis information
+       and closure environments *)
+    ArgRelIP : onv val -> onv val -> A-> list val -> list val -> Prop;
+    (* Relates environments according to analysis information *)
+    ArgLengthMatchIP : forall E E' a Z Z' VL VL',
+        ParamRelIP a Z Z' -> ArgRelIP E E' a VL VL' -> length Z = length VL /\ length Z' = length VL';
+}.
+
+Lemma pointwise_PR_as_PR A
+  : PointwiseProofRelationI A -> ProofRelationI A.
 Proof.
-  assert (forall n n', IndexRelI (AL' ++ AL) n n' -> n < length F -> n' < length F').
-  intros. rewrite IDX in H. subst; omega.
-  assert (forall n n', IndexRelI (AL' ++ AL) n n' -> n >= length F -> n' >= length F').
-  intros. rewrite IDX in H0. subst; omega.
-  intros. eapply simILabenv_extension'; eauto.
+  intros. destruct X as [B C D].
+  eapply (Build_ProofRelationI B C (fun _ => eq) (@length _) D).
+  intros; eauto.
+Defined.
+
+Lemma IndexRelIP_eq A PR L n n'
+  : @IndexRelI A (pointwise_PR_as_PR PR) L n n' <-> n = n'.
+Proof.
+  destruct PR; simpl. reflexivity.
+Qed.
+
+Hint Resolve pointwise_PR_as_PR : typeclass_instances.
+
+Coercion pointwise_PR_as_PR : PointwiseProofRelationI >-> ProofRelationI.
+
+
+Lemma labenv_sim_extension_ptw t A (PR:PointwiseProofRelationI A) (AL AL':list A) F F' L L'
+  : (forall r ,
+        labenv_sim t (sim'r r) PR (AL' ++ AL) (mapi I.mkBlock F ++ L) (mapi I.mkBlock F' ++ L')
+        -> indexwise_r t (sim'r r) PR AL' F F' AL (mapi I.mkBlock F ++ L) (mapi I.mkBlock F' ++ L'))
+    -> indexwise_paramrel PR F F' AL' AL
+    -> length AL' = length F
+    -> length F = length F'
+    -> forall r, labenv_sim t (sim'r r) PR AL L L'
+        -> labenv_sim t (sim'r r) PR (AL' ++ AL) (mapi I.mkBlock F ++ L) (mapi I.mkBlock F' ++ L').
+Proof.
+  intros ISIM IP Len1 Len2 r SIML.
+  assert (separates PR AL' AL F F'). {
+    destruct SIML; dcr.
+    hnf; destruct PR; simpl; repeat split; intros; omega.
+  }
+  eapply labenv_sim_extension'; eauto.
   eapply indexwise_r_mon.
-  eapply fix_compatible_I; eauto. eauto.
+  eapply fix_compatible_separate; eauto. eauto.
 Qed.
